src/Backends/Boogie/Compiler.dfy
@@ -1,0 +1,395 @@
+include "../../Interop/CSharpDafnyASTModel.dfy"
+include "../../Interop/CSharpInterop.dfy"
+include "../../Interop/CSharpDafnyInterop.dfy"
+include "../../AST/Translator.dfy"
+include "../../Passes/EliminateNegatedBinops.dfy"
+include "../../Transforms/BottomUp.dfy"
+include "../../Utils/Library.dfy"
+include "../../Utils/StrTree.dfy"
+include "../../../../../../BoogieV/lang/BoogieLang.dfy"
+
+module {:extern "Bootstrap.Backends.Boogie.Compiler"} {:options "-functionSyntax:4"}
+  Bootstrap.Backends.Boogie
+{
+  import opened Interop.CSharpDafnyInterop
+  import opened AST.Syntax
+  import AST.Predicates
+  import Passes.EliminateNegatedBinops
+  import opened AST.Predicates.Deep
+  import opened Utils.Lib.Datatypes
+  import Transforms.BottomUp
+  import Transforms.Generic
+  import BV = BoogieLang
+  import BLib = Wrappers
+
+  type WfExpr = e: Exprs.T | Deep.All_Expr(e, Exprs.WellFormed) witness *
+
+  function CompileLiteralExpr(l: Exprs.Literal) : BV.Expr
+    requires l.LitInt? || l.LitBool?
+  {
+    match l {
+      case LitBool(b) => BV.ELit(BV.LitBool(b))
+      case LitInt(i) => BV.ELit(BV.LitInt(i))
+    }
+  }
+
+  function CompileLazyExpr(op: Exprs.LazyOp, e0: BV.Expr, e1: BV.Expr) : BV.Expr {
+    var bop := match op
+      case And => BV.Binop.And
+      case Or => BV.Binop.Or
+      case Imp => BV.Binop.Imp;
+    BV.BinOp(e0, bop, e1)
+  }
+
+  function CompileUnaryOpExpr(op: UnaryOp, e: BV.Expr) : BV.Expr {
+    var uop := match op
+      case BoolNot() => BV.Not
+      case BVNot() => Crash("BVNot")
+      case SeqLength() => Crash("SeqLength")
+      case SetCard() => Crash("SetCard")
+      case MultisetCard() => Crash("MultisetCard")
+      case MapCard() => Crash("MapCard")
+      case MemberSelect(_) => Crash("MemberSelect");
+    BV.UnOp(uop, e)
+  }
+
+  function CompileBinaryExpr(op: BinaryOp, e0: BV.Expr, e1: BV.Expr) : BV.Expr {
+    var bop := match op
+      case Logical(Iff) => BV.Iff
+
+      case Eq(EqCommon) => BV.Eq
+      case Eq(NeqCommon) => BV.Neq
+
+      case Numeric(Lt) => BV.Lt
+      case Numeric(Le) => BV.Le
+      case Numeric(Ge) => BV.Ge
+      case Numeric(Gt) => BV.Gt
+      case Numeric(Add) => BV.Add
+      case Numeric(Sub) => BV.Sub
+      case Numeric(Mul) => BV.Mul
+      case Numeric(Div) => BV.Div
+      case Numeric(Mod) => BV.Mod
+
+      case _ => Crash("BinOp");
+    BV.BinOp(e0, bop, e1)
+  }
+
+  function Crash<A>(msg: string): (a: A) {
+    assume false;
+    Crash(msg)
+  } by method {
+    print msg;
+    expect false;
+    a := Crash(msg);
+  }
+
+  function Annotated<A, T>(a: A, annot: T): A {
+    a
+  }
+
+  predicate SupportsVerification_Expr(e: Expr) {
+    Exprs.WellFormed(e) &&
+    match e {
+      case Var(x) => true
+      case Literal(l) =>
+        l.LitInt? || l.LitBool?
+      case Abs(_, _) =>
+        Annotated(false, "Expr.Abs")
+      case Apply(op, es) =>
+        && (forall e <- es :: SupportsVerification_Expr(e))
+        && match op {
+            case Lazy(op) => true
+            case Eager(UnaryOp(op)) => true
+            case Eager(BinaryOp(op)) => true
+            case Eager(TernaryOp(op)) => Annotated(false, "Expr.TernaryOp")
+            case Eager(Builtin(Display(ty))) => Annotated(false, "Expr.Builtin(Display)")
+            case Eager(Builtin(Progn)) => Annotated(false, "Expr.Builtin(Progn)")
+            case Eager(Builtin(Assert)) => Annotated(false, "Expr.Builtin(Assert)")
+            case Eager(Builtin(Print)) => Annotated(false, "Expr.Builtin(Print)")
+            case Eager(DataConstructor(name, typeArgs)) => Annotated(false, "Expr.DataConstructor")
+            case Eager(FunctionCall()) => Annotated(false, "Expr.FunctionCall")
+          }
+      case Block(exprs) =>
+        Annotated(false, "Expr.Block")
+      case Bind(vars, vals, body) =>
+        && |vars| == |vals| == 1
+        && (forall e <- vals :: SupportsVerification_Expr(e))
+        && SupportsVerification_Expr(body)
+      case If(cond, thn, els) =>
+        Annotated(false, "Expr.If")
+    }
+  }
+
+  predicate SupportsVerification_Stmt(s: Expr) {
+    match s {
+      case Var(_) => Annotated(false, "Stmt.Var")
+      case Literal(l) => Annotated(false, "Stmt.Literal")
+      case Abs(_, _) => Annotated(false, "Stmt.Abs")
+      case Apply(op, es) =>
+        match op {
+          case Eager(Builtin(Assert)) => (forall e <- es :: SupportsVerification_Expr(e))
+          case Eager(Builtin(Progn)) => (forall e <- es :: SupportsVerification_Stmt(e))
+          case _ => Annotated(false, "Stmt.Apply")
+        }
+      case Block(exprs) =>
+        && (forall e <- exprs :: SupportsVerification_Stmt(e))
+      case Bind(vars, vals, body) =>
+        && |vars| == |vals| == 1
+        && (forall e <- vals :: SupportsVerification_Expr(e))
+        && SupportsVerification_Stmt(body)
+      case If(cond, thn, els) =>
+        && SupportsVerification_Expr(cond)
+        && SupportsVerification_Stmt(thn)
+        && SupportsVerification_Stmt(els)
+    }
+  }
+
+  // FIXME(CPC): Predicate to characterize supported terms?
+
+  function CompileExpr(e: WfExpr) : BV.Expr
+    requires SupportsVerification_Expr(e)
+    decreases e, 0
+  {
+    match e {
+      case Var(x) =>
+        BV.Var(x)
+      case Literal(l) =>
+        CompileLiteralExpr(l)
+      case Apply(op, es) =>
+        match op {
+          case Lazy(op) =>
+            var c0, c1 := CompileExpr(es[0]), CompileExpr(es[1]);
+            CompileLazyExpr(op, c0, c1)
+          case Eager(UnaryOp(op)) =>
+            CompileUnaryOpExpr(op, CompileExpr(es[0]))
+          case Eager(BinaryOp(op)) =>
+            CompileBinaryExpr(op, CompileExpr(es[0]), CompileExpr(es[1]))
+        }
+      case Bind(vars, vals, body) =>
+        assert |vars| == |vals| == 1;
+        var decls := Seq.Map(x requires x in vars => (x, BV.Ty.TPrim(BV.PrimTy.TInt)), vars);
+        BV.Let(vars[0], CompileExpr(vals[0]), CompileExpr(body))
+    }
+  }
+
+  function CompileStmt(e: WfExpr) : BV.Cmd
+    requires SupportsVerification_Stmt(e)
+    decreases e, 0
+  {
+    match e {
+      case Apply(op, args) =>
+        match op {
+          case Eager(Builtin(Assert)) =>
+            BV.SimpleCmd(BV.Assert(CompileExpr(args[0])))
+          case Eager(Builtin(Progn)) =>
+            var bexprs := Seq.Map(x requires x in args => CompileStmt(x), args);
+            Seq.FoldR((acc, x) => BV.Seq(x, acc), BV.SimpleCmd(BV.Skip), bexprs)
+        }
+      case Block(exprs) =>
+        var bexprs := Seq.Map(x requires x in exprs => CompileStmt(x), exprs);
+        Seq.FoldR((acc, x) => BV.Seq(x, acc), BV.SimpleCmd(BV.Skip), bexprs)
+      case Bind(vars, vals, body) =>
+        // TODO: Assumes all variables are int
+        var decls := Seq.Map(x requires x in vars => (x, BV.Ty.TPrim(BV.PrimTy.TInt)), vars);
+        BV.Scope(labelName := BLib.None, varDecls := decls, body := CompileStmt(body))
+      case If(cond, thn, els) =>
+        BV.If(BLib.Some(CompileExpr(cond)), CompileStmt(thn), CompileStmt(els))
+    }
+  }
+
+  function WellFormednessAssertion1(e: WfExpr): Option<WfExpr>
+  {
+    Predicates.Deep.AllImpliesChildren(e, Exprs.WellFormed);
+    match e {
+      case Var(_) => None
+      case Literal(l) => None
+      case Abs(_, _) => None
+      case Apply(Lazy(op), es) => None
+      case Apply(Eager(op), es) =>
+        match op {
+          case BinaryOp(Numeric(Div)) => Some(Neq(es[1], Zero))
+          case _ => None
+        }
+      case Block(es) => None
+      case Bind(vars, es, body) => None
+      case If(cond, thn, els) => None
+    }
+  }
+
+  function AddAssertion(assertion: WfExpr, e: WfExpr): (e': WfExpr) {
+    Progn([Assert(assertion), e])
+  }
+
+  function AddWellFormednessAssertions1(e: WfExpr): (e': WfExpr) {
+    match WellFormednessAssertion1(e)
+      case Some(wf) => AddAssertion(wf, e)
+      case None => e
+  }
+
+  const AddWellFormednessAssertionsTR: BottomUp.BottomUpTransformer :=
+    assume false; Generic.TR(AddWellFormednessAssertions1, _ => true);
+
+  // FIXME move / remove?
+  function ReplaceChildren(e: Expr, children: seq<Expr>): (e': Expr)
+    requires |children| == |e.Children()|
+  {
+    match e {
+      case Var(_) => e
+      case Literal(lit) => e
+      case Abs(vars, body) => Exprs.Abs(vars, children[0])
+      case Apply(aop, exprs) => Exprs.Apply(aop, children)
+      case Block(exprs) => Exprs.Block(children)
+      case Bind(vars, vals, body) =>
+        Exprs.Bind(vars, children[..|children| - 1], children[|children| - 1])
+      case If(cond, thn, els) =>
+        Exprs.If(children[0], children[1], children[2])
+    }
+  }
+
+  function RemoveProgns1(e: Expr): (e': Expr)
+  {
+    if e.Apply? && e.aop == OpProgn && |e.args| == 1 then e.args[0]
+    else e
+  }
+
+  const RemovePrognTR: BottomUp.BottomUpTransformer :=
+    assume false; Generic.TR(RemoveProgns1, _ => true)
+
+  const True: WfExpr :=
+    Exprs.Literal(Exprs.LitBool(true))
+  const Zero: WfExpr :=
+    Exprs.Literal(Exprs.LitInt(0))
+  const And: (WfExpr, WfExpr) -> WfExpr :=
+    (a, b) => Exprs.Apply(Exprs.Lazy(Exprs.And), [a, b])
+  const Imp: (WfExpr, WfExpr) -> WfExpr :=
+    (a, b) => Exprs.Apply(Exprs.Lazy(Exprs.Imp), [a, b])
+  const Not: (WfExpr) -> WfExpr :=
+    (a) => Exprs.Apply(Exprs.Eager(Exprs.UnaryOp(UnaryOps.BoolNot)), [a])
+  const Neq: (WfExpr, WfExpr) -> WfExpr :=
+    (a, b) => Exprs.Apply(Exprs.Eager(Exprs.BinaryOp(BinaryOps.Eq(BinaryOps.NeqCommon))), [a, b])
+  const OpAssert :=
+    Exprs.Eager(Exprs.Builtin(Exprs.Assert))
+  const Assert: (WfExpr) -> WfExpr :=
+    (e) => Exprs.Apply(OpAssert, [e])
+  const OpProgn :=
+    Exprs.Eager(Exprs.Builtin(Exprs.Progn))
+  const Progn: (seq<WfExpr>) --> WfExpr :=
+    (es) requires |es| > 0 => var wf: WfExpr := Exprs.Apply(OpProgn, es); wf
+
+  function RemoveNone<A>(opts: seq<Option<A>>): seq<A> {
+    if |opts| == 0 then []
+    else if opts[0].Some? then [opts[0].value] + RemoveNone(opts[1..])
+    else RemoveNone(opts[1..])
+  }
+
+  function Unzip<A, B>(zipped: seq<(A, B)>): (p: (seq<A>, seq<B>))
+    ensures |p.0| == |p.1| == |zipped|
+  {
+    if |zipped| == 0 then ([], [])
+    else
+      var (sA, sB) := Unzip(zipped[1..]);
+      (([zipped[0].0] + sA), ([zipped[0].1] + sB))
+  }
+
+  function PeelOffAssert(e: WfExpr): (e': (Option<WfExpr>, WfExpr)) {
+    Predicates.Deep.AllImpliesChildren(e, Exprs.WellFormed);
+    if e.Apply? && e.aop == OpProgn && |e.args| > 1 then
+      var fst: Expr := e.args[0];
+      Predicates.Deep.AllImpliesChildren(fst, Exprs.WellFormed);
+      if fst.Apply? && fst.aop == OpAssert then
+          assert |fst.args| == 1;
+          (Some(fst.args[0]), Progn(e.args[1..]))
+      else (None, e)
+    else (None, e)
+  }
+
+  function PeelOffAsserts(es: seq<WfExpr>): (pairs: (seq<Option<WfExpr>>, seq<WfExpr>))
+    ensures |pairs.0| == |pairs.1| == |es|
+  {
+    Unzip(Seq.Map(e requires e in es => PeelOffAssert(e), es))
+  }
+
+  function MergeAsserts(wfs: seq<WfExpr>): (wf: WfExpr) {
+    if |wfs| == 0 then True
+    else if |wfs| == 1 then wfs[0]
+    else And(wfs[0], MergeAsserts(wfs[1..]))
+  }
+
+  function AddAssertions(wfs: seq<WfExpr>, e: WfExpr): (e': WfExpr) {
+    if |wfs| == 0 then e
+    else AddAssertion(MergeAsserts(wfs), e)
+  }
+
+  function LiftAsserts1(e: WfExpr): (e': WfExpr) {
+    match e {
+      case Var(_) => e
+      case Literal(lit) => e
+      case Abs(vars, body) =>
+        Crash<WfExpr>("LiftAssert.Abs")
+      case Apply(op, exprs) =>
+        var (wfs, exprs) := PeelOffAsserts(exprs);
+        var wfs := match op {
+          case Lazy(And) | Lazy(Imp) =>
+            [wfs[0], wfs[1].Map(wf => Imp(exprs[0], wf))]
+          case Lazy(Or) =>
+            [wfs[0], wfs[1].Map(wf => Imp(Not(exprs[0]), wf))]
+          case _ => wfs
+        };
+        AddAssertions(RemoveNone(wfs), Exprs.Apply(op, exprs))
+      case Block(exprs) =>
+        var (wfs, exprs) := PeelOffAsserts(exprs);
+        AddAssertions(RemoveNone(wfs), Exprs.Block(exprs))
+      case Bind(vars, vals, body) =>
+        var (wfs_vals, vals) := PeelOffAsserts(vals);
+        var (wf_body, body) := PeelOffAssert(body);
+        var wf_body: Option<WfExpr> := wf_body.Map(wf => Exprs.Bind(vars, vals, wf));
+        AddAssertions(RemoveNone(wfs_vals + [wf_body]), Exprs.Bind(vars, vals, body))
+      case If(cond, thn, els) =>
+        var (wf_cond, cond) := PeelOffAssert(cond);
+        var (wf_thn, thn) := PeelOffAssert(thn);
+        var (wf_els, els) := PeelOffAssert(els);
+        var wf_thn := wf_thn.Map(wf => Imp(cond, wf));
+        var wf_els := wf_els.Map(wf => Imp(Not(cond), wf));
+        AddAssertions(RemoveNone([wf_cond, wf_thn, wf_els]), Exprs.If(cond, thn, els))
+    }
+  }
+
+  const LiftAssertsTR: BottomUp.BottomUpTransformer :=
+    assume false; Generic.TR(LiftAsserts1, _ => true)
+
+  function CompileMethod(m: Method) : BV.Cmd
+    requires Deep.All_Method(m, Exprs.WellFormed)
+    requires Shallow.All_Method(m, SupportsVerification_Stmt)
+  {
+    match m {
+      case Method(nm, methodBody) => CompileStmt(methodBody)
+    }
+  }
+
+  function CompileProgram(p: Program) : BV.Cmd
+    requires Deep.All_Program(p, Exprs.WellFormed)
+    requires Shallow.All_Program(p, SupportsVerification_Stmt)
+  {
+    match p {
+      case Program(mainMethod) => CompileMethod(mainMethod)
+    }
+  }
+
+  method VerifyProgram(p: Program) returns (st: BV.Cmd)
+  {
+    if Deep.All_Program(p, Exprs.WellFormed) {
+      var p :=
+        assume false;
+        var p := BottomUp.Map_Program(p, AddWellFormednessAssertionsTR);
+        var p := BottomUp.Map_Program(p, LiftAssertsTR);
+        var p := BottomUp.Map_Program(p, RemovePrognTR);
+        p;
+
+      if Shallow.All_Program(p, SupportsVerification_Stmt) {
+        print CompileProgram(p).ToString(indent := 0);
+      }
+    } else {
+      print "Well-formedness check failed.";
+    }
+  }
+}
