src/Backends/Boogie/tmp.dfy
@@ -1,0 +1,30 @@
+include "../../Interop/CSharpDafnyASTModel.dfy"
+include "../../Interop/CSharpInterop.dfy"
+include "../../Interop/CSharpDafnyInterop.dfy"
+include "../../AST/Translator.dfy"
+include "../../Passes/EliminateNegatedBinops.dfy"
+include "../../Transforms/BottomUp.dfy"
+include "../../Utils/Library.dfy"
+include "../../Utils/StrTree.dfy"
+include "../../../../../../BoogieV/lang/BoogieLang.dfy"
+
+module {:extern "Bootstrap.Backends.Boogie.Compiler"} {:options "-functionSyntax:4"}
+  Bootstrap.Backends.Boogie
+{
+  import opened Interop.CSharpDafnyInterop
+  import opened AST.Syntax
+  import AST.Predicates
+  import Passes.EliminateNegatedBinops
+  import opened AST.Predicates.Deep
+  import opened Utils.Lib.Datatypes
+  import Transforms.BottomUp
+  import Transforms.Generic
+  import BV = BoogieLang
+  import BLib = Wrappers
+
+  type WfExpr = e: Exprs.T | Deep.All_Expr(e, Exprs.WellFormed) witness *
+  const OpProgn :=
+    Exprs.Eager(Exprs.Builtin(Exprs.Progn))
+  const Progn: (seq<WfExpr>) --> WfExpr :=
+    (es) requires |es| > 0 => var r: WfExpr := Exprs.Apply(OpProgn, es); r
+}
